internal/examples/semantics/int_conversions.go
@@ -1,0 +1,23 @@
+package semantics
+
+func testU64ToU32() bool {
+	var ok = true
+	x := uint64(1230)
+	y := uint32(1230)
+	ok = ok && uint32(x) == y
+	ok = ok && uint64(y) == x
+	return ok
+}
+
+func testU32Len() bool {
+	s := make([]byte, 100)
+	return uint32(len(s)) == uint32(100)
+}
+
+type Uint32 uint32
+
+// https://github.com/tchajed/goose/issues/14
+func failing_testU32NewtypeLen() bool {
+	s := make([]byte, 20)
+	return Uint32(len(s)) == Uint32(20)
+}
